Make Seq changes

src/Collections/Sequences/Seq.dfy
@@ -223,7 +223,7 @@ module Seq {
     requires v in s
     ensures i < |s| && s[i] == v
   {
-    if s[|s|-1] == v then |s| - 1 else IndexOf(s[..|s|-1], v)
+    if s[0] == v then 0 else 1 + IndexOf(s[1..], v)
   }
 
   /* finds the index of a certain element in the sequence if found */
@@ -260,40 +260,22 @@ module Seq {
       s[..i] + s[i+1..]
   }
 
-  /* slices out a specific value from the sequence if found */
-  function method {:opaque} RemoveValueOption<T(==)>(s: seq<T>, o: Option<T>): (s': seq<T>)
-    ensures o == None || (|s| == 0 && |s'| == 0) ||
-      (|s| > 0 && var v := o.UnwrapOr(s[0]);
-        v !in s ==> s == s'
-        && v in s ==> |multiset(s')| == |multiset(s)| - 1
-        && v in s ==> multiset(s')[v] == multiset(s)[v] - 1
-        && HasNoDuplicates(s) ==> HasNoDuplicates(s') && ToSet(s') == ToSet(s) - {v})
-  {
-    reveal HasNoDuplicates();
-    reveal ToSet();
-    match o
-    case None => s
-    case Some(v) =>
-      if v !in s then s else
-      var i := IndexOf(s, v);
-      assert s == s[..i] + [v] + s[i+1..];
-      s[..i] + s[i+1..]
-  }
-
   /* inserts a certain value into a specified index of the sequence */
   function method {:opaque} Insert<T>(s: seq<T>, a: T, pos: nat): seq<T>
-    requires pos <= |s|;
-    ensures |Insert(s, a, pos)| == |s| + 1;
-    ensures forall i {:trigger Insert(s, a, pos)[i], s[i]}:: 0 <= i < pos ==> Insert(s, a, pos)[i] == s[i];
-    ensures forall i {:trigger s[i]} :: pos <= i < |s| ==> Insert(s, a, pos)[i+1] == s[i];
-    ensures Insert(s, a, pos)[pos] == a;
+    requires pos <= |s|
+    ensures |Insert(s, a, pos)| == |s| + 1
+    ensures forall i {:trigger Insert(s, a, pos)[i], s[i]} :: 0 <= i < pos ==> Insert(s, a, pos)[i] == s[i]
+    ensures forall i {:trigger s[i]} :: pos <= i < |s| ==> Insert(s, a, pos)[i+1] == s[i]
+    ensures Insert(s, a, pos)[pos] == a
     ensures multiset(Insert(s, a, pos)) == multiset(s) + multiset{a}
   {
     assert s == s[..pos] + s[pos..];
     s[..pos] + [a] + s[pos..]
   }
 
-  function method {:opaque} Reverse<T>(s: seq<T>): seq<T>
+  function method {:opaque} Reverse<T>(s: seq<T>): (s': seq<T>)
+    ensures |s'| == |s|
+    ensures forall i {:trigger s'[i]}{:trigger s[|s| - i - 1]} :: 0 <= i < |s| ==> s'[i] == s[|s| - i - 1]
   {
     if s == [] then [] else [s[|s|-1]] + Reverse(s[0 .. |s|-1])
   }
@@ -322,13 +304,12 @@ module Seq {
 
   /* takes two sequences, a and b, and combines then to form one sequence in which
   each position contains an ordered pair from a and b */
-  function method {:opaque} Zip<A,B>(a: seq<A>, b: seq<B>): seq<(A,B)>
+  function method {:opaque} Zip<A,B>(a: seq<A>, b: seq<B>): seq<(A, B)>
     requires |a| == |b|
-    ensures |
-    Zip(a, b)| == |a|
+    ensures |Zip(a, b)| == |a|
     ensures forall i {:trigger Zip(a, b)[i]}:: 0 <= i < |Zip(a, b)| ==> Zip(a, b)[i] == (a[i], b[i])
-    ensures Unzip(Zip(a, b)).0 == a;
-    ensures Unzip(Zip(a, b)).1 == b;
+    ensures Unzip(Zip(a, b)).0 == a
+    ensures Unzip(Zip(a, b)).1 == b
   {
     if |a| == 0 then []
     else Zip(DropLast(a), DropLast(b)) + [(Last(a), Last(b))]
@@ -552,7 +533,7 @@ module Seq {
   /* concatenating two sequences and then applying Map is the same as applying
   Map on each sequence  seperately and then concatenating the two resulting
   sequences */
-  lemma {:opaque} LemmaMapAndConcatCommute<T,R>(f: (T ~> R), a: seq<T>, b: seq<T>)
+  lemma {:opaque} LemmaMapDistributesOverConcat<T,R>(f: (T ~> R), a: seq<T>, b: seq<T>)
     requires forall i {:trigger a[i]}:: 0 <= i < |a| ==> f.requires(a[i])
     requires forall j {:trigger b[j]}:: 0 <= j < |b| ==> f.requires(b[j])
     ensures Map(f, a + b) == Map(f, a) + Map(f, b)
@@ -585,7 +566,7 @@ module Seq {
 
   /* concatenating two sequences and then using "filter" is the same as using "filter" on each sequences
   seperately and then concatenating their resulting sequences */
-  lemma {:opaque} LemmaFilterAndCommute<T>(f: (T ~> bool), a: seq<T>, b: seq<T>)
+  lemma {:opaque} LemmaFilterDistributesOverConcat<T>(f: (T ~> bool), a: seq<T>, b: seq<T>)
     requires forall i {:trigger a[i]}:: 0 <= i < |a| ==> f.requires(a[i])
     requires forall j {:trigger b[j]}:: 0 <= j < |b| ==> f.requires(b[j])
     ensures Filter(f, a + b) == Filter(f, a) + Filter(f, b)
@@ -613,7 +594,7 @@ module Seq {
 
   /* Concatenating two sequences, then folding left is the same as folding the first sequence and using the result as the initial value to fold the second
   sequence. */
-  lemma {:opaque} LemmaFoldLeftConcatAndCommute<A,T>(f: (A, T) -> A, init: A, a: seq<T>, b: seq<T>)
+  lemma {:opaque} LemmaFoldLeftDistributesOverConcat<A,T>(f: (A, T) -> A, init: A, a: seq<T>, b: seq<T>)
     requires 0 <= |a + b|
     ensures FoldLeft(f, init, a + b) == FoldLeft(f, FoldLeft(f, init, a), b)
   {
@@ -626,7 +607,7 @@ module Seq {
       calc {
         FoldLeft(f, FoldLeft(f, init, a), b);
         FoldLeft(f, FoldLeft(f, f(init, a[0]), a[1..]), b);
-          { LemmaFoldLeftConcatAndCommute(f, f(init, a[0]), a[1..], b); }
+          { LemmaFoldLeftDistributesOverConcat(f, f(init, a[0]), a[1..], b); }
         FoldLeft(f, f(init, a[0]), a[1..] + b);
           { assert (a + b)[0] == a[0];
             assert (a + b)[1..] == a[1..] + b; }
@@ -671,7 +652,7 @@ module Seq {
 
   /* Concatenating two sequences, then folding right is the same as folding the second sequence and using the result as the initial value to fold the first
   sequence. */
-  lemma {:opaque} LemmaFoldRightConcatAndCommute<A,T>(f: (T, A) -> A, init: A, a: seq<T>, b: seq<T>)
+  lemma {:opaque} LemmaFoldRightDistributesOverConcat<A,T>(f: (T, A) -> A, init: A, a: seq<T>, b: seq<T>)
     requires 0 <= |a + b|
     ensures FoldRight(f, a + b, init) == FoldRight(f, a, FoldRight(f, b, init))
   {
